theories/case_studies/generator_iterator.v
@@ -22,18 +22,13 @@ From affine_tes.logic Require Import sem_operators.
 From affine_tes.logic Require Import tactics.
 From affine_tes.logic Require Import compatibility.
 
-From affine_tes.case_studies Require Import representable.
-From affine_tes.case_studies Require Import iterator.
-From affine_tes.case_studies Require Import generator.
-From affine_tes.case_studies Require Import ghost.
-
 Definition yield := (λ: "x", perform: "x")%V.
 Definition generate :=
   (λ: "i", let: "cont" := ref (λ: <>, "i" <_> yield) in
-           λ: <>, let: "comp" := Load "cont" in
+      λ: <>, let: "comp" := "cont" <!- (λ: <>, #())  in
              shallow-try-os: "comp" #() with
                 effect λ: "w" "k", "cont" <- "k" ;; SOME "w"
-             |  return λ: "w", "cont" <- (λ: <>,  #()) ;; NONE
+             |  return λ: "w", NONE
              end
   )%V.
 
@@ -50,59 +45,50 @@ Section typing.
 
   Context `{!heapGS Σ}.
 
-  Definition yield_sig (τ : sem_ty Σ) := (∀μTS: _, _, τ ⇒ ())%R.
-  Definition yield_ty τ := τ -{ yield_sig τ }-> ().
+  Definition yield_sig (τ : sem_ty Σ) := (μ∀TS: _, _, τ ⇒ ())%R.
+  Definition yield_ty τ := τ -{ ⟨yield_sig τ,⟩ }-> ().
   Definition iter_ty τ := (∀R: θ, (τ -{ θ }-> ()) -{ θ }-∘ ())%T.
-  Definition generator_ty τ := (() >-∘ Option τ)%T.
+  Definition generator_ty τ := (() → Option τ)%T.
   
   Lemma sem_typed_generate τ :
     ⊢ ⊨ᵥ generate : (iter_ty τ → generator_ty τ).
   Proof.
     iIntros "". iApply sem_typed_closure; first done.
-    iApply (sem_typed_let _ [("i", iter_ty τ)] _ _ _ _ (yield_ty τ)); solve_sidecond. 
-    - iApply sem_typed_val. iApply sem_typed_closure; first done.
-      iApply (sem_typed_perform _ _ _ () with "[]"). 
-      iApply sem_typed_sub_nil.
-      iApply sem_typed_var.
-    - set cont_ty := Ref (() -{ yield_sig τ }-∘ ()). 
-      iApply (sem_typed_let _ [] _ _ _ _ cont_ty); solve_sidecond.
-      + set Γ₁ :=[("yield", yield_ty τ); ("i", iter_ty τ)].
-        iApply sem_typed_alloc.
-        rewrite -(app_nil_r Γ₁).
-        iApply sem_typed_afun; solve_sidecond. simpl.
-        iApply (sem_typed_app _ [("i", iter_ty τ)]);
-          last (iApply sem_typed_sub_nil; iApply sem_typed_var).
-        iApply (sem_typed_SApp _ _ _ (yield_sig τ) (λ ρ, ( τ -{ ρ }-> ()) -{ ρ }-∘ ())).
-        iApply sem_typed_sub_nil. 
-        iApply sem_typed_var.
-      + set Γ₁ :=[("cont", cont_ty)]; rewrite -(app_nil_r Γ₁). 
-        set in_cont_ty := (() -{ yield_sig τ }-∘ ()).
-        iApply sem_typed_sufun; solve_sidecond.
-        iApply (sem_typed_let _ [("cont", Ref Moved)] _ _ _ _ in_cont_ty); solve_sidecond.
-        { iApply sem_typed_sub_nil. iApply sem_typed_load. }
-        rewrite app_singletons.
-        iPoseProof (sem_typed_shallow_try 
-                      [("comp", in_cont_ty)] [] [("cont", cont_ty)] 
-                      [("cont", Ref Moved)]
-                      "w" "k" _ _ _ (λ _ _, τ) (λ _ _, ()) (Option τ) ()) as "Hhand"; solve_sidecond.
-        rewrite /Γ₁. iApply "Hhand"; iClear "Hhand".
-        * iApply sem_typed_app; iApply sem_typed_sub_nil;
+    set cont_ty := (() -{ ⟨yield_sig τ,⟩ }-∘ ()). 
+    iApply (sem_typed_let _ [] _ _ _ _ (Refᶜ cont_ty)); simpl; solve_sidecond. 
+    - iApply sem_typed_alloc_cpy.
+      rewrite -(app_nil_r [("i", _)]).
+      iApply sem_typed_afun; solve_sidecond. simpl.
+      iApply (sem_typed_app _ [("i", iter_ty τ)] _ _ _ (yield_ty τ)); solve_sidecond.
+      + iApply (sem_typed_SApp _ _ _ ⟨yield_sig τ,⟩%R (λ ρ, ( τ -{ ρ }-> ()) -{ ρ }-∘ ())); solve_sidecond.
+        iApply sem_typed_sub_nil. iApply sem_typed_var.
+      + iApply sem_typed_frame_os. iApply sem_typed_sub_nil.
+        iApply sem_typed_val. iApply sem_typed_closure; first done.
+        simpl. iApply (sem_typed_perform_os _ _ _ () with "[]"). 
+        iApply sem_typed_sub_nil. iApply sem_typed_var.
+    - set Γ₁ :=[("cont", Refᶜ cont_ty)]; rewrite -(app_nil_r Γ₁). 
+      iApply sem_typed_ufun; solve_sidecond. simpl.
+      iApply (sem_typed_let _ [("cont", Refᶜ cont_ty)] _ _ _ _ cont_ty); solve_sidecond.
+      + iApply sem_typed_contraction; solve_sidecond.
+        iApply sem_typed_replace_cpy.
+        { iApply sem_typed_sub_nil. iApply sem_typed_var. }
+        do 2 iApply sem_typed_frame_os.
+        rewrite -(app_nil_r []).
+        iApply sem_typed_afun; solve_sidecond.
+        simpl. iApply sem_typed_sub_nil. iApply sem_typed_unit.
+      + rewrite app_singletons.
+        iApply (sem_typed_shallow_try_os' 
+                      [("comp", cont_ty)] [] [] [("cont", Refᶜ cont_ty)] 
+                      "w" "k" _ _ _ (λ _ _, τ) (λ _ _, ()) (Option τ) ()); solve_sidecond.
+        * iApply sem_typed_app; first solve_sidecond; 
+          iApply sem_typed_sub_nil;
             [iApply sem_typed_var|iApply sem_typed_unit]. 
-        * iIntros (?). iApply sem_typed_swap_third.
-          iApply sem_typed_seq.
-          { iApply sem_typed_store. 
-            iApply sem_typed_swap_third.
-            iApply sem_typed_var. }
-          iApply sem_typed_swap_second.
+        * iIntros (?). do 2 iApply sem_typed_swap_third.
+          iApply (sem_typed_seq _ [("w", τ)]).
+          { iApply (sem_typed_store_cpy _ _ _ _ _ _ cont_ty); iApply sem_typed_var. }
           iApply sem_typed_some.
           iApply sem_typed_var.
-        * iApply sem_typed_weaken.
-          iApply sem_typed_seq. 
-          iApply sem_typed_store.
-          { rewrite -(app_nil_l [("cont", Ref Moved)]).
-            iApply sem_typed_afun; solve_sidecond.
-            iApply sem_typed_sub_nil.
-            iApply sem_typed_unit. }
+        * simpl. do 2 iApply sem_typed_weaken.
           iApply sem_typed_none.
   Qed.
   
@@ -111,157 +97,31 @@ Section typing.
   Proof.
     iIntros. iApply sem_typed_closure; first done. rewrite /iter_ty /=.
     rewrite - {1}(app_nil_r [("g", _)]). 
-    iApply sem_typed_SLam. iIntros (ρ).
+    iApply sem_typed_SLam; solve_sidecond. iIntros (θ).
     rewrite - {1}(app_nil_r [("g", _)]). 
     iApply sem_typed_sub_nil. 
-    iApply sem_typed_afun; solve_sidecond.
-    iApply sem_typed_app;
+    iApply sem_typed_afun; solve_sidecond. simpl.
+    iApply sem_typed_app; first solve_sidecond;
       [|iApply sem_typed_sub_nil; iApply sem_typed_swap_second; iApply sem_typed_var].
-      rewrite - {1}((app_nil_r [("f", _)])). 
-    iApply sem_typed_sub_ty; [apply ty_le_u2aarr|].
+    rewrite - {1}((app_nil_r [("f", _)])). 
+    iApply sem_typed_sub_ty; [iApply ty_le_u2aarr|].
     iApply sem_typed_sub_nil.
-    iApply sem_typed_ufun; solve_sidecond.
-    set Γ₂ := [("g", generator_ty τ); ("go", generator_ty τ -{ ρ }-> () ); ("f", τ -{ ρ }-> ())].
-    iApply (sem_typed_match_option _ Γ₂ _ _ _ _ _ () _ τ); solve_sidecond.
+    iApply sem_typed_ufun; solve_sidecond. simpl.
+    set Γ₂ := [("g", generator_ty τ); ("go", generator_ty τ -{ θ }-> () ); ("f", τ -{ θ }-> ())].
+    iApply (sem_typed_match_option _ Γ₂ _ _ _ _ _ θ τ); solve_sidecond.
     - iApply sem_typed_sub_nil. 
-      iApply sem_typed_suapp. iApply sem_typed_unit.
-    - iApply sem_typed_sub_nil. do 3 (iApply sem_typed_weaken). iApply sem_typed_unit.
-    - iApply sem_typed_seq.
-      + iApply sem_typed_app; [|iApply sem_typed_sub_nil; iApply sem_typed_var].
+      iApply sem_typed_app; solve_sidecond; last iApply sem_typed_unit.
+      iApply sem_typed_contraction; solve_sidecond. 
+      iApply sem_typed_sub_nil. 
+      iApply sem_typed_sub_ty; [iApply ty_le_u2aarr|iApply sem_typed_var].
+    - iApply sem_typed_sub_nil. do 3 iApply sem_typed_weaken. iApply sem_typed_unit.
+    - iApply (sem_typed_seq _ [("g", generator_ty τ ); ("go", generator_ty τ -{ θ }-> ())]).
+      + iApply sem_typed_app; [solve_sidecond| |iApply sem_typed_sub_nil; iApply sem_typed_var].
         iApply sem_typed_sub_nil. iApply sem_typed_swap_third. 
-        iApply sem_typed_sub_ty; [apply ty_le_u2aarr|]. iApply sem_typed_var.
-      + iApply sem_typed_app; [|iApply sem_typed_sub_nil; iApply sem_typed_var].
-        iApply sem_typed_sub_nil. iApply sem_typed_sub_ty; [apply ty_le_u2aarr|].
+        iApply sem_typed_sub_ty; [iApply ty_le_u2aarr|]. iApply sem_typed_var.
+      + iApply sem_typed_app; [solve_sidecond| |iApply sem_typed_sub_nil; iApply sem_typed_var].
+        iApply sem_typed_sub_nil. iApply sem_typed_sub_ty; [iApply ty_le_u2aarr|].
         iApply sem_typed_var.
   Qed.
 
 End typing.
-
-Section verification.
-    Context `{!heapGS Σ}.
-    Context {G : Type → Type} `{DataStructure Σ G, Iterable G}.
-    Context {A : Type} `{Representable Σ A}.
-    Context `{!inG Σ (excl_authR (leibnizO (list A)))}.
-
-    Definition isIterCont (l : loc) γ (us : list A) (T : G A) : iProp Σ :=
-      ∃ k, l ↦ k ∗ handlerView γ us ∗
-                   EWP k #() <| YIELD (iterView γ) T |> {{ _, ∃ us, ⌜complete T us⌝ ∗ (iterView γ) us }}.
-
-    Lemma generate_spec_iter_cont (l : loc) γ (us : list A) (T : G A) :
-      let e := 
-        (λ: <>, 
-          let: "comp" := Load #l in
-                shallow-try: "comp" #() with 
-                  effect (λ: "w" "k", #l <- "k";; InjR "w")
-                | return (λ: "w", #l <- (λ: <>, #());; InjL #())
-                end)%V in
-      isIterCont l γ us T -∗ isGen e T us.
-    Proof. 
-      simpl. iLöb as "IH" forall (us).
-      iIntros "(%k & Hl & Hhand & Hk)".
-      rewrite isGen_unfold /isGen_pre.
-      ewp_pure_steps. ewp_bind_rule. iApply (ewp_load with "Hl").
-      iIntros "!> Hl !> /=". ewp_pure_steps. 
-      iApply (ewp_try_with with "Hk").
-      iSplit; [|iSplit; iIntros (v c)];
-      last (iIntros "?"; by rewrite upcl_bottom).
-      - iIntros (v) "(%us' & %Hcompl & Hiter)".
-        ewp_pure_steps. ewp_bind_rule. iApply (ewp_store with "Hl").
-        iIntros "!> Hl !> /=". ewp_pure_steps. 
-        iDestruct (confront_views with "Hhand Hiter") as %->.
-        iSplitR; [by iPureIntro|].
-        iApply "IH". rewrite /isIterCont.
-        iExists (λ: <>, #())%V. iFrame. ewp_pure_steps. iFrame.
-        iExists us. iFrame. by iPureIntro.
-      - rewrite upcl_yield.
-        iIntros "(%us' & %u & %x & -> & (Hxu & %Hperm & Hiter) & HQ)".
-        ewp_pure_steps. ewp_bind_rule. iApply (ewp_store with "Hl").
-        iDestruct (confront_views with "Hhand Hiter") as %->.
-        iIntros "!> Hl".
-        iMod (update_cell _ (us ++ [u]) with "Hhand Hiter") as "[Hhand Hiter]".
-        iIntros "!> /=". ewp_pure_steps. iExists u. iFrame. 
-        iSplit; [by iPureIntro|].
-        iApply "IH". rewrite /isIterCont. iExists c. iFrame.
-        iApply ("HQ" with "[Hiter]"). iFrame.
-    Qed.
-
-  Lemma generate_spec (i : val) (T : G A) :
-    isIter i T -∗ EWP (generate i) {{ g, isGen g T [] }}.
-  Proof.
-    iIntros "Hi". rewrite /generate.
-    ewp_pure_steps. ewp_bind_rule. simpl.
-    iApply ewp_alloc. iIntros "!> %l Hl".
-    iMod (new_cell []) as (γ) "[Hhand Hiter]".
-    iIntros "!>". ewp_pure_steps.
-    iAssert (isIterCont l γ [] T) with "[Hl Hi Hhand Hiter]" as "H";
-    last (by iApply generate_spec_iter_cont).
-    rewrite /isIterCont. iExists (λ: <>, i #() (λ: "x", perform:"x")%V)%V.
-    iFrame. rewrite /isIter.
-    set I := (iterView γ).
-    iSpecialize ("Hi" $! (YIELD I T) yield I). rewrite /I.
-    ewp_pure_steps. rewrite -/yield. iApply ("Hi" with "[] Hiter").
-    iIntros "!# %us %u %v %Hperm Hrepr Hiter".
-    rewrite /yield /rec_perform. ewp_pure_steps. iApply ewp_do_os.
-    rewrite upcl_yield. iExists us,u,v. iSplitR; first done.
-    iFrame. iSplitR; first done. 
-    iIntros "Hiter". by ewp_pure_steps.
-  Qed.
-
-  Lemma iterate_spec_helper uus g (f : val) Ψ I (T : G A) :
-    □ (∀ (us : list A) (u : A) (v : val),
-          ⌜permitted T (us ++ [u])⌝ -∗
-          represents v u -∗ I us -∗ EWP f v <| Ψ |> {{ _, I (us ++ [u]) }}) -∗
-    isGen g T uus -∗
-    I uus -∗
-    EWP (rec: "go" "g" :=
-          match: "g" #() with InjL <> => #() | InjR "x" => f "x";; "go" "g" end)%V g
-          <| Ψ |> {{ _, ∃ us : list A, ⌜complete T us⌝ ∗ I us }}.
-  Proof. 
-    iIntros "#Hf Hgen HI".
-    iLöb as "IH" forall (uus). 
-    rewrite isGen_unfold /isGen_pre; ewp_pure_steps; ewp_bind_rule; 
-    iApply (ewp_mono with "[Hgen]"); 
-      try (iApply ewp_os_prot_mono; [iApply iEff_le_bottom|iApply "Hgen"]); 
-      iIntros "%v Hv !> /="; destruct v eqn:Hv; try done; ewp_pure_steps. 
-    - iExists uus. iFrame.
-      destruct v0; try done. destruct l; try done.
-      by iDestruct "Hv" as "[Hcompl _]". 
-    - ewp_bind_rule. 
-      iDestruct "Hv" as "(%u & Hrepr & Hperm & Hgen)".
-      iApply (ewp_mono with "[Hf Hperm Hrepr HI]").
-      { iApply ("Hf" $! uus with "Hperm Hrepr HI"). }
-      iIntros (w) "HI !> /=". do 3 ewp_value_or_step.
-      iApply ("IH" $! (uus ++ [u]) with "Hgen HI").
-  Qed.
-
-  Lemma iterate_spec g (T : G A) :
-    isGen g T [] -∗ EWP (iterate g) {{ i, isIter i T }}.
-  Proof.
-    iIntros "Hgen". rewrite /iterate. ewp_pure_steps.
-    rewrite /isIter. iIntros (Ψ f I) "#Hf HI". 
-    do 6 ewp_value_or_step. 
-    iApply (iterate_spec_helper [] with "Hf Hgen HI").
-  Qed.
-
-  Lemma generate_iterate_inv i (T : G A) :
-    isIter i T -∗ EWP iterate (generate i) {{ i, isIter i T }}.
-  Proof.
-    iIntros "Hi". ewp_bind_rule.
-    iApply (ewp_mono with "[Hi]"). 
-    { iApply (generate_spec with "Hi"). }
-    iIntros (g) "Hg !> /=".
-    by iApply iterate_spec.
-  Qed.
-
-
-  Lemma iterate_generate_inv g (T : G A) :
-    isGen g T [] -∗ EWP generate (iterate g) {{ g, isGen g T [] }}.
-  Proof.
-    iIntros "Hg". ewp_bind_rule.
-    iApply (ewp_mono with "[Hg]"). 
-    { iApply (iterate_spec with "Hg"). }
-    iIntros (i) "Hi !> /=".
-    by iApply generate_spec.
-  Qed.
-    
-End verification.
