theories/case_studies/state.v
@@ -128,8 +128,7 @@ Section typing.
     rewrite app_singletons.
     set A := (λ (_ : sem_sig Σ) (_ : sem_ty Σ), (@sem_ty_unit Σ) + ℤ)%T.
     set B := (λ (_ : sem_sig Σ) (_ : sem_ty Σ), @sem_ty_int Σ)%T.
-    iApply sem_typed_sub_env_final; [iApply env_le_weaken|].
-    iApply (sem_typed_deep_try_os' _ [] _ "x" _ _ _ _ A B ℤ _ (@sem_sig_nil Σ) with "[] [] []"); solve_sidecond.
+    iApply (sem_typed_deep_try_os' _ [] _ _ "x" _ _ _ _ A B ℤ _ (@sem_sig_nil Σ) with "[] [] []"); solve_sidecond.
     { rewrite /A /B -/stsig. 
       iApply sem_typed_app; first solve_copy; iApply sem_typed_sub_nil; 
       last (iApply sem_typed_var).
@@ -141,9 +140,6 @@ Section typing.
       + iApply sem_typed_app; first solve_copy; [iApply sem_typed_var|].
         iApply (sem_typed_load_cpy _ _ _ _ ℤ); solve_sidecond.
         iApply sem_typed_swap_second. 
-        iApply sem_typed_contraction; solve_sidecond.
-        iApply sem_typed_swap_third. 
-        iApply sem_typed_swap_second. 
         iApply sem_typed_var.
       + iApply sem_typed_swap_third. iApply sem_typed_contraction; solve_sidecond.
         iApply sem_typed_swap_third.
@@ -152,12 +148,8 @@ Section typing.
             solve_sidecond; iApply sem_typed_var. }
         iApply sem_typed_app; [solve_copy|iApply sem_typed_var|].
         iApply (sem_typed_load_cpy _ _ _ _ ℤ); solve_sidecond.
-        iApply sem_typed_contraction; solve_sidecond.
-        iApply sem_typed_swap_third. 
-        iApply sem_typed_swap_second. 
         iApply sem_typed_var.
     - simpl. iApply sem_typed_weaken. iApply sem_typed_load_cpy; solve_sidecond.
-      iApply sem_typed_contraction; solve_sidecond.
       iApply sem_typed_var.
   Qed.
 
@@ -169,7 +161,7 @@ Section typing.
     set A := (λ (_ : sem_sig Σ) (_ : sem_ty Σ), (@sem_ty_unit Σ) + ℤ)%T.
     set B := (λ (_ : sem_sig Σ) (_ : sem_ty Σ), @sem_ty_int Σ)%T.
     rewrite - {1} (app_nil_r [("n", ℤ)]).
-    iApply (sem_typed_deep_try_os' _ [] _ _ _ _ _ _ A B); solve_sidecond.
+    iApply (sem_typed_deep_try_os' _ [] _ _ _ _ _ _ _ A B); solve_sidecond.
     { rewrite /A /B -/stsig. 
       iApply sem_typed_app; first solve_copy; iApply sem_typed_sub_nil; 
       last (iApply sem_typed_var).
